checker/theories/Typing.v
@@ -1275,7 +1275,7 @@ Proof.
     cbn in IH'; forward IH'. constructor 1; cbn. lia.
     apply IH'; auto.
   - simpl. simpl in *.
-    destruct g; simpl.
+    destruct d.
     + destruct c; simpl in *.
       destruct cst_body; simpl in *.
       simpl.
@@ -1598,12 +1598,12 @@ Qed.
 Lemma lookup_on_global_env `{checker_flags} P Σ c decl :
   on_global_env P Σ ->
   lookup_env Σ c = Some decl ->
-  { Σ' & { wfΣ' : on_global_env P Σ'.1 & on_global_decl P Σ' decl } }.
+  { Σ' & { wfΣ' : on_global_env P Σ'.1 & on_global_decl P Σ' c decl } }.
 Proof.
   induction 1; simpl.
   congruence.
-  destruct ident_eq.
-  - intros [= ->].
+  destruct (ident_eq_spec c kn).
+  - intros [= ->]. subst c.
     exists (Σ, udecl). constructor; tas.
   - apply IHX.
 Qed.
