template-coq/theories/Pretty.v
@@ -83,23 +83,17 @@ Section print_term.
          | nAnon => true
          end) Γ.
 
-  Definition global_decl_ident d :=
-    match d with
-    | ConstantDecl id _ => id
-    | InductiveDecl id _ => id
-    end.
-
   Fixpoint lookup_env (Σ : global_env) (id : ident) : option global_decl :=
     match Σ with
     | nil => None
     | hd :: tl =>
-      if ident_eq id (global_decl_ident hd) then Some hd
+      if ident_eq id hd.1 then Some hd.2
       else lookup_env tl id
     end.
 
   Definition lookup_ind_decl ind i :=
     match lookup_env Σ ind with
-    | Some (InductiveDecl _ {| ind_bodies := l; ind_universes := uctx |}) =>
+    | Some (InductiveDecl {| ind_bodies := l; ind_universes := uctx |}) =>
       match nth_error l i with
       | Some body => Some body
       | None => None
